% Generated by GrindEQ Word-to-LaTeX 
\documentclass{article} %%% use \documentstyle for old LaTeX compilers

\usepackage[english]{babel} %%% 'french', 'german', 'spanish', 'danish', etc.
\usepackage{amssymb}
\usepackage{amsmath}
\usepackage{txfonts}
\usepackage{mathdots}
\usepackage[classicReIm]{kpfonts}
\usepackage[dvips]{graphicx} %%% use 'pdftex' instead of 'dvips' for PDF output

% You can include more LaTeX packages here 


\begin{document}

%\selectlanguage{english} %%% remove comment delimiter ('%') and select language if required


\noindent 证明
\[{\rm Z} (2)=\sum _{n=1}^{\infty }\frac{1}{n^{2} }  =\frac{\pi ^{2} }{6} \] 
\#\# 思路一

\noindent 

\noindent 利用傅里叶级数

\noindent 

\noindent \#\#\# 探索 1

\noindent 
\[\#\#\#\# {\rm Z} (2)=\frac{\pi ^{2} }{6} \] 


\noindent $f(x)=x^{2} $ ， 傅里叶展开后得

\noindent 
\[f(x)=\frac{\pi ^{2} }{3} +\sum _{n=1}^{\infty }\left((-1)^{n} \frac{4}{n^{2} } \cos nx\right) \] 


\noindent 考虑要消掉 $(-1)^{n} $ ，注意到 $\cos (n\pi )=(-1)^{n} $

\noindent 

\noindent 令 $x=\pi ,\pi ^{2} =g(\pi )=\frac{\pi ^{2} }{3} +4\sum _{n=1}^{\infty }\left(\frac{1}{n^{2} } \right) \Rightarrow \sum _{n=1}^{\infty }\left(\frac{1}{n^{2} } \right) =\frac{\pi ^{2} }{6} $

\noindent 
\[\#\#\#\# {\rm Z} (4)=\frac{\pi ^{4} }{90} \] 


\noindent $x^{4} $ 展开后得

\noindent 
\[x^{4} =\frac{\pi ^{4} }{5} +\sum _{n=1}^{\infty }\frac{8(-1)^{n} \left(\pi ^{2} n^{2} -6\right)}{n^{4} }  \cos (nx)\] 


\noindent 取 $x=\pi $

\noindent 
\[\pi ^{4} =\frac{\pi ^{4} }{5} +\sum _{n=1}^{\infty }\frac{8\left(\pi ^{2} n^{2} -6\right)}{n^{4} }  =\frac{\pi ^{4} }{5} +\sum _{n=1}^{\infty }\left(\frac{8\pi ^{2} }{n^{2} } -\frac{48}{n^{4} } \right) \] 


\noindent 利用 ${\rm Z} \eqref{GrindEQ__2_}=\frac{\pi ^{2} }{6} $ 即证

\noindent 
\[\#\#\#\# {\rm Z} (6)=\frac{\pi ^{6} }{945} \] 


\noindent $x^{6} $ 展开后得

\noindent 
\[x^{6} =\frac{\pi ^{6} }{7} +\sum _{n=1}^{\infty }\frac{12(-1)^{n} \left(\pi ^{4} n^{4} -20\pi ^{2} n^{2} +120\right)}{n^{6} }  \cos (nx)\] 

\[x=\pi \] 

\[\pi ^{6} =\frac{\pi ^{6} }{7} +\sum _{n=1}^{\infty }\left(\frac{1440}{n^{6} } -\frac{240\pi ^{2} }{n^{4} } +\frac{12\pi ^{4} }{n^{2} } \right) \] 


\noindent 利用 ${\rm Z} \eqref{GrindEQ__2_}=\frac{\pi ^{2} }{6} ,{\rm Z} \eqref{GrindEQ__4_}=\frac{\pi ^{4} }{90} $ 即证

\noindent 
\[\#\#\#\# {\rm Z} (8)=\frac{\pi ^{8} }{9450} \] 


\noindent $x^{8} $ 展开后得

\noindent 
\[x^{8} =\frac{\pi ^{8} }{9} +\sum _{n=1}^{\infty }\frac{16(-1)^{n} \left(\pi ^{6} n^{6} -42\pi ^{4} n^{4} +840\pi ^{2} n^{2} -5040\right)}{n^{8} }  \cos (nx)\] 
\[x=\pi \] 
\[\pi ^{8} =\frac{\pi ^{8} }{9} +\sum _{n=1}^{\infty }\left(-\frac{80640}{n^{8} } +\frac{13440\pi ^{2} }{n^{6} } -\frac{672\pi ^{4} }{n^{4} } +\frac{16\pi ^{6} }{n^{2} } \right) \] 


\noindent 同理易证

\noindent 

\noindent \#\# 思路二

\noindent 

\noindent 计算 
\[\int _{0}^{1}\int _{0}^{1}\frac{1}{1-xy}   {\kern 1pt} {\rm d}x{\kern 1pt} {\rm d}y\] 


\noindent \#\#\# 探索 2

\noindent 

\noindent 证明 $\frac{1}{1-xy} $ 在 $[0,1]\times [0,1]$ 内的积分与 $(0,1)\times (0,1)$ 的积分值相同

\noindent 
\[\oint _{L}\frac{1}{1-xy}  {\kern 1pt} {\rm d}s\] 


\noindent 其中 $L$ 是顶点为 $(0,0),(0,1),(1,1),(1,0)$ 的正方形的正向边界

\noindent 

\noindent 四条边分开积分

\noindent 
\[\int _{0}^{1}\frac{1}{1-y}  {\kern 1pt} {\rm d}y+\int _{1}^{0}1 {\kern 1pt} {\rm d}y+\int _{0}^{1}1 {\kern 1pt} {\rm d}x+\int _{1}^{0}\frac{1}{1-x}  {\kern 1pt} {\rm d}x=0\] 



\end{document}

